qcp/ast/VC/thm_apply_goal.v
@@ -1483,6 +1483,668 @@ forall (l: (@list term)) (tail_ptr: Z) ,
   **  (sll_term_list check_list l )
 .
 
+(*----- Function thm_apply -----*)
+
+Definition thm_apply_safety_wit_1 := 
+forall (goal_pre: Z) (lis_pre: Z) (thm_pre: Z) (X: (solve_res -> (unit -> Prop))) (g: term) (l: (@list var_sub)) (t: term) (retval: Z) (retval_2: Z) (v: Z) (res_type: Z) ,
+  [| (res_type = 0) |] 
+  &&  [| (v = 0) |] 
+  &&  [| (retval_2 <> 0) |] 
+  &&  [| (thm_pre <> 0) |] 
+  &&  [| (safeExec ATrue (thm_app_rel (t) (l) (g)) X ) |]
+  &&  ((( &( "res" ) )) # Ptr  |-> retval_2)
+  **  ((&((retval_2)  # "solve_res" ->ₛ "type")) # Int  |-> res_type)
+  **  ((&((retval_2)  # "solve_res" ->ₛ "d" .ₛ "ans")) # Int  |-> v)
+  **  (sll_var_sub_list lis_pre l )
+  **  (store_sub_thm_res thm_pre retval t l )
+  **  ((( &( "thm_ins" ) )) # Ptr  |-> retval)
+  **  ((( &( "goal" ) )) # Ptr  |-> goal_pre)
+  **  ((( &( "lis" ) )) # Ptr  |-> lis_pre)
+  **  ((( &( "thm" ) )) # Ptr  |-> thm_pre)
+  **  (store_term goal_pre g )
+|--
+  [| (0 <= INT_MAX) |] 
+  &&  [| ((INT_MIN) <= 0) |]
+.
+
+Definition thm_apply_safety_wit_2 := 
+forall (goal_pre: Z) (lis_pre: Z) (thm_pre: Z) (X: (solve_res -> (unit -> Prop))) (g: term) (l: (@list var_sub)) (t: term) (retval: Z) (retval_2: Z) (v: Z) (res_type: Z) ,
+  [| (retval = 0) |] 
+  &&  [| (res_type = 0) |] 
+  &&  [| (v = 0) |] 
+  &&  [| (retval_2 <> 0) |] 
+  &&  [| (thm_pre <> 0) |] 
+  &&  [| (safeExec ATrue (thm_app_rel (t) (l) (g)) X ) |]
+  &&  ((( &( "res" ) )) # Ptr  |-> retval_2)
+  **  ((&((retval_2)  # "solve_res" ->ₛ "type")) # Int  |-> res_type)
+  **  ((&((retval_2)  # "solve_res" ->ₛ "d" .ₛ "ans")) # Int  |-> v)
+  **  (sll_var_sub_list lis_pre l )
+  **  (store_sub_thm_res thm_pre retval t l )
+  **  ((( &( "thm_ins" ) )) # Ptr  |-> retval)
+  **  ((( &( "goal" ) )) # Ptr  |-> goal_pre)
+  **  ((( &( "lis" ) )) # Ptr  |-> lis_pre)
+  **  ((( &( "thm" ) )) # Ptr  |-> thm_pre)
+  **  (store_term goal_pre g )
+|--
+  [| (0 <= INT_MAX) |] 
+  &&  [| ((INT_MIN) <= 0) |]
+.
+
+Definition thm_apply_safety_wit_3 := 
+forall (goal_pre: Z) (lis_pre: Z) (thm_pre: Z) (X: (solve_res -> (unit -> Prop))) (g: term) (l: (@list var_sub)) (t: term) (retval: Z) (retval_2: Z) (v: Z) (res_type: Z) ,
+  [| (retval = 0) |] 
+  &&  [| (res_type = 0) |] 
+  &&  [| (v = 0) |] 
+  &&  [| (retval_2 <> 0) |] 
+  &&  [| (thm_pre <> 0) |] 
+  &&  [| (safeExec ATrue (thm_app_rel (t) (l) (g)) X ) |]
+  &&  ((( &( "res" ) )) # Ptr  |-> retval_2)
+  **  ((&((retval_2)  # "solve_res" ->ₛ "type")) # Int  |-> 0)
+  **  ((&((retval_2)  # "solve_res" ->ₛ "d" .ₛ "ans")) # Int  |-> v)
+  **  (sll_var_sub_list lis_pre l )
+  **  (store_sub_thm_res thm_pre retval t l )
+  **  ((( &( "thm_ins" ) )) # Ptr  |-> retval)
+  **  ((( &( "goal" ) )) # Ptr  |-> goal_pre)
+  **  ((( &( "lis" ) )) # Ptr  |-> lis_pre)
+  **  ((( &( "thm" ) )) # Ptr  |-> thm_pre)
+  **  (store_term goal_pre g )
+|--
+  [| (0 <= INT_MAX) |] 
+  &&  [| ((INT_MIN) <= 0) |]
+.
+
+Definition thm_apply_safety_wit_4 := 
+forall (goal_pre: Z) (lis_pre: Z) (thm_pre: Z) (X: (solve_res -> (unit -> Prop))) (g: term) (l: (@list var_sub)) (t: term) (retval_2: Z) (retval_3: Z) (v: Z) (res_type: Z) (pq: partial_quant) (st: term) (retval: Z) ,
+  [| (retval <> 0) |] 
+  &&  [| (retval = (term_alpha_eqn (st) (g))) |] 
+  &&  [| (thm_subst_allres_rel t l pq st ) |] 
+  &&  [| (retval_2 <> 0) |] 
+  &&  [| (res_type = 0) |] 
+  &&  [| (v = 0) |] 
+  &&  [| (retval_3 <> 0) |] 
+  &&  [| (thm_pre <> 0) |] 
+  &&  [| (safeExec ATrue (thm_app_rel (t) (l) (g)) X ) |]
+  &&  (store_term retval_2 st )
+  **  (store_term goal_pre g )
+  **  ((( &( "thm_ins" ) )) # Ptr  |-> retval_2)
+  **  ((( &( "thm" ) )) # Ptr  |-> thm_pre)
+  **  (store_partial_quant thm_pre retval_2 pq )
+  **  ((( &( "res" ) )) # Ptr  |-> retval_3)
+  **  ((&((retval_3)  # "solve_res" ->ₛ "type")) # Int  |-> res_type)
+  **  ((&((retval_3)  # "solve_res" ->ₛ "d" .ₛ "ans")) # Int  |-> v)
+  **  (sll_var_sub_list lis_pre l )
+  **  ((( &( "goal" ) )) # Ptr  |-> goal_pre)
+  **  ((( &( "lis" ) )) # Ptr  |-> lis_pre)
+|--
+  [| (0 <= INT_MAX) |] 
+  &&  [| ((INT_MIN) <= 0) |]
+.
+
+Definition thm_apply_safety_wit_5 := 
+forall (goal_pre: Z) (lis_pre: Z) (thm_pre: Z) (X: (solve_res -> (unit -> Prop))) (g: term) (l: (@list var_sub)) (t: term) (retval_2: Z) (retval_3: Z) (v: Z) (res_type: Z) (pq: partial_quant) (st: term) (retval: Z) ,
+  [| (retval <> 0) |] 
+  &&  [| (retval = (term_alpha_eqn (st) (g))) |] 
+  &&  [| (thm_subst_allres_rel t l pq st ) |] 
+  &&  [| (retval_2 <> 0) |] 
+  &&  [| (res_type = 0) |] 
+  &&  [| (v = 0) |] 
+  &&  [| (retval_3 <> 0) |] 
+  &&  [| (thm_pre <> 0) |] 
+  &&  [| (safeExec ATrue (thm_app_rel (t) (l) (g)) X ) |]
+  &&  (store_term retval_2 st )
+  **  (store_term goal_pre g )
+  **  ((( &( "thm_ins" ) )) # Ptr  |-> retval_2)
+  **  ((( &( "thm" ) )) # Ptr  |-> thm_pre)
+  **  (store_partial_quant thm_pre retval_2 pq )
+  **  ((( &( "res" ) )) # Ptr  |-> retval_3)
+  **  ((&((retval_3)  # "solve_res" ->ₛ "type")) # Int  |-> 0)
+  **  ((&((retval_3)  # "solve_res" ->ₛ "d" .ₛ "ans")) # Int  |-> v)
+  **  (sll_var_sub_list lis_pre l )
+  **  ((( &( "goal" ) )) # Ptr  |-> goal_pre)
+  **  ((( &( "lis" ) )) # Ptr  |-> lis_pre)
+|--
+  [| (1 <= INT_MAX) |] 
+  &&  [| ((INT_MIN) <= 1) |]
+.
+
+Definition thm_apply_safety_wit_6 := 
+forall (goal_pre: Z) (lis_pre: Z) (thm_pre: Z) (X: (solve_res -> (unit -> Prop))) (g: term) (l: (@list var_sub)) (t: term) (retval_2: Z) (retval_3: Z) (v: Z) (res_type: Z) (pq: partial_quant) (st: term) (retval: Z) ,
+  [| (retval = 0) |] 
+  &&  [| (retval = (term_alpha_eqn (st) (g))) |] 
+  &&  [| (thm_subst_allres_rel t l pq st ) |] 
+  &&  [| (retval_2 <> 0) |] 
+  &&  [| (res_type = 0) |] 
+  &&  [| (v = 0) |] 
+  &&  [| (retval_3 <> 0) |] 
+  &&  [| (thm_pre <> 0) |] 
+  &&  [| (safeExec ATrue (thm_app_rel (t) (l) (g)) X ) |]
+  &&  (store_term retval_2 st )
+  **  (store_term goal_pre g )
+  **  ((( &( "thm_ins" ) )) # Ptr  |-> retval_2)
+  **  ((( &( "thm" ) )) # Ptr  |-> thm_pre)
+  **  (store_partial_quant thm_pre retval_2 pq )
+  **  ((( &( "res" ) )) # Ptr  |-> retval_3)
+  **  ((&((retval_3)  # "solve_res" ->ₛ "type")) # Int  |-> res_type)
+  **  ((&((retval_3)  # "solve_res" ->ₛ "d" .ₛ "ans")) # Int  |-> v)
+  **  (sll_var_sub_list lis_pre l )
+  **  ((( &( "goal" ) )) # Ptr  |-> goal_pre)
+  **  ((( &( "lis" ) )) # Ptr  |-> lis_pre)
+|--
+  [| (1 <= INT_MAX) |] 
+  &&  [| ((INT_MIN) <= 1) |]
+.
+
+Definition thm_apply_return_wit_1_1 := 
+forall (goal_pre: Z) (lis_pre: Z) (thm_pre: Z) (X: (solve_res -> (unit -> Prop))) (g: term) (l: (@list var_sub)) (t_3: term) (retval_3: Z) (retval: Z) (v: Z) (res_type: Z) (pq: partial_quant) (st: term) (retval_4: Z) (v_2: Z) (retval_5: Z) (R: ((term * (@list term)) -> (unit -> Prop))) (t_2: term) (l_2: (@list term)) (retval_2: Z) ,
+  [| (safeExec ATrue (ret ((makepair (t_2) (l_2)))) R ) |] 
+  &&  [| (safeExec ATrue (check_rel (st) (g)) R ) |] 
+  &&  [| (retval_5 <> 0) |] 
+  &&  [| (v_2 = 0) |] 
+  &&  [| (retval_4 = 0) |] 
+  &&  [| (retval_4 = (term_alpha_eqn (st) (g))) |] 
+  &&  [| (thm_subst_allres_rel t_3 l pq st ) |] 
+  &&  [| (retval_3 <> 0) |] 
+  &&  [| (res_type = 0) |] 
+  &&  [| (v = 0) |] 
+  &&  [| (retval <> 0) |] 
+  &&  [| (thm_pre <> 0) |] 
+  &&  [| (safeExec ATrue (thm_app_rel (t_3) (l) (g)) X ) |]
+  &&  (store_term goal_pre g )
+  **  (sll_term_list retval_2 l_2 )
+  **  (store_term retval_3 st )
+  **  ((&((retval)  # "solve_res" ->ₛ "d" .ₛ "list")) # Ptr  |-> retval_2)
+  **  (store_partial_quant thm_pre retval_3 pq )
+  **  ((&((retval)  # "solve_res" ->ₛ "type")) # Int  |-> 1)
+  **  (sll_var_sub_list lis_pre l )
+|--
+  EX (t: term)  (sr: solve_res) ,
+  [| (safeExec ATrue (ret (sr)) X ) |]
+  &&  (store_term thm_pre t )
+  **  (sll_var_sub_list lis_pre l )
+  **  (store_term goal_pre g )
+  **  (store_solve_res retval sr )
+.
+
+Definition thm_apply_return_wit_1_2 := 
+forall (goal_pre: Z) (lis_pre: Z) (thm_pre: Z) (X: (solve_res -> (unit -> Prop))) (g: term) (l: (@list var_sub)) (t_2: term) (retval_3: Z) (retval: Z) (v: Z) (res_type: Z) (pq: partial_quant) (st: term) (retval_2: Z) ,
+  [| (retval_2 <> 0) |] 
+  &&  [| (retval_2 = (term_alpha_eqn (st) (g))) |] 
+  &&  [| (thm_subst_allres_rel t_2 l pq st ) |] 
+  &&  [| (retval_3 <> 0) |] 
+  &&  [| (res_type = 0) |] 
+  &&  [| (v = 0) |] 
+  &&  [| (retval <> 0) |] 
+  &&  [| (thm_pre <> 0) |] 
+  &&  [| (safeExec ATrue (thm_app_rel (t_2) (l) (g)) X ) |]
+  &&  (store_term retval_3 st )
+  **  (store_term goal_pre g )
+  **  (store_partial_quant thm_pre retval_3 pq )
+  **  ((&((retval)  # "solve_res" ->ₛ "type")) # Int  |-> 0)
+  **  ((&((retval)  # "solve_res" ->ₛ "d" .ₛ "ans")) # Int  |-> 1)
+  **  (sll_var_sub_list lis_pre l )
+|--
+  EX (t: term)  (sr: solve_res) ,
+  [| (safeExec ATrue (ret (sr)) X ) |]
+  &&  (store_term thm_pre t )
+  **  (sll_var_sub_list lis_pre l )
+  **  (store_term goal_pre g )
+  **  (store_solve_res retval sr )
+.
+
+Definition thm_apply_return_wit_1_3 := 
+forall (goal_pre: Z) (lis_pre: Z) (thm_pre: Z) (X: (solve_res -> (unit -> Prop))) (g: term) (l: (@list var_sub)) (t_2: term) (retval_2: Z) (retval: Z) (v: Z) (res_type: Z) ,
+  [| (retval_2 = 0) |] 
+  &&  [| (res_type = 0) |] 
+  &&  [| (v = 0) |] 
+  &&  [| (retval <> 0) |] 
+  &&  [| (thm_pre <> 0) |] 
+  &&  [| (safeExec ATrue (thm_app_rel (t_2) (l) (g)) X ) |]
+  &&  ((&((retval)  # "solve_res" ->ₛ "type")) # Int  |-> 0)
+  **  ((&((retval)  # "solve_res" ->ₛ "d" .ₛ "ans")) # Int  |-> 0)
+  **  (sll_var_sub_list lis_pre l )
+  **  (store_sub_thm_res thm_pre retval_2 t_2 l )
+  **  (store_term goal_pre g )
+|--
+  EX (t: term)  (sr: solve_res) ,
+  [| (safeExec ATrue (ret (sr)) X ) |]
+  &&  (store_term thm_pre t )
+  **  (sll_var_sub_list lis_pre l )
+  **  (store_term goal_pre g )
+  **  (store_solve_res retval sr )
+.
+
+Definition thm_apply_partial_solve_wit_1 := 
+forall (goal_pre: Z) (lis_pre: Z) (thm_pre: Z) (X: (solve_res -> (unit -> Prop))) (g: term) (l: (@list var_sub)) (t: term) ,
+  [| (thm_pre <> 0) |] 
+  &&  [| (safeExec ATrue (thm_app_rel (t) (l) (g)) X ) |]
+  &&  (store_term thm_pre t )
+  **  (sll_var_sub_list lis_pre l )
+  **  (store_term goal_pre g )
+|--
+  [| (thm_pre <> 0) |] 
+  &&  [| (safeExec ATrue (thm_app_rel (t) (l) (g)) X ) |]
+  &&  (store_term thm_pre t )
+  **  (sll_var_sub_list lis_pre l )
+  **  (store_term goal_pre g )
+.
+
+Definition thm_apply_partial_solve_wit_2 := 
+forall (goal_pre: Z) (lis_pre: Z) (thm_pre: Z) (X: (solve_res -> (unit -> Prop))) (g: term) (l: (@list var_sub)) (t: term) (retval: Z) ,
+  [| (thm_pre <> 0) |] 
+  &&  [| (safeExec ATrue (thm_app_rel (t) (l) (g)) X ) |]
+  &&  (sll_var_sub_list lis_pre l )
+  **  (store_sub_thm_res thm_pre retval t l )
+  **  (store_term goal_pre g )
+|--
+  [| (thm_pre <> 0) |] 
+  &&  [| (safeExec ATrue (thm_app_rel (t) (l) (g)) X ) |]
+  &&  (sll_var_sub_list lis_pre l )
+  **  (store_sub_thm_res thm_pre retval t l )
+  **  (store_term goal_pre g )
+.
+
+Definition thm_apply_partial_solve_wit_3 := 
+forall (goal_pre: Z) (lis_pre: Z) (thm_pre: Z) (X: (solve_res -> (unit -> Prop))) (g: term) (l: (@list var_sub)) (t: term) (retval: Z) (retval_2: Z) ,
+  [| (retval_2 <> 0) |] 
+  &&  [| (thm_pre <> 0) |] 
+  &&  [| (safeExec ATrue (thm_app_rel (t) (l) (g)) X ) |]
+  &&  (store_solve_res retval_2 (SRBool (0)) )
+  **  (sll_var_sub_list lis_pre l )
+  **  (store_sub_thm_res thm_pre retval t l )
+  **  (store_term goal_pre g )
+|--
+  [| (retval_2 <> 0) |] 
+  &&  [| (thm_pre <> 0) |] 
+  &&  [| (safeExec ATrue (thm_app_rel (t) (l) (g)) X ) |]
+  &&  (store_solve_res retval_2 (SRBool (0)) )
+  **  (sll_var_sub_list lis_pre l )
+  **  (store_sub_thm_res thm_pre retval t l )
+  **  (store_term goal_pre g )
+.
+
+Definition thm_apply_partial_solve_wit_4_pure := 
+forall (goal_pre: Z) (lis_pre: Z) (thm_pre: Z) (X: (solve_res -> (unit -> Prop))) (g: term) (l: (@list var_sub)) (t: term) (retval: Z) (retval_2: Z) (v: Z) (res_type: Z) ,
+  [| (retval <> 0) |] 
+  &&  [| (res_type = 0) |] 
+  &&  [| (v = 0) |] 
+  &&  [| (retval_2 <> 0) |] 
+  &&  [| (thm_pre <> 0) |] 
+  &&  [| (safeExec ATrue (thm_app_rel (t) (l) (g)) X ) |]
+  &&  ((( &( "res" ) )) # Ptr  |-> retval_2)
+  **  ((&((retval_2)  # "solve_res" ->ₛ "type")) # Int  |-> res_type)
+  **  ((&((retval_2)  # "solve_res" ->ₛ "d" .ₛ "ans")) # Int  |-> v)
+  **  (sll_var_sub_list lis_pre l )
+  **  (store_sub_thm_res thm_pre retval t l )
+  **  ((( &( "thm_ins" ) )) # Ptr  |-> retval)
+  **  ((( &( "goal" ) )) # Ptr  |-> goal_pre)
+  **  ((( &( "lis" ) )) # Ptr  |-> lis_pre)
+  **  ((( &( "thm" ) )) # Ptr  |-> thm_pre)
+  **  (store_term goal_pre g )
+|--
+  [| (retval <> 0) |]
+.
+
+Definition thm_apply_partial_solve_wit_4_aux := 
+forall (goal_pre: Z) (lis_pre: Z) (thm_pre: Z) (X: (solve_res -> (unit -> Prop))) (g: term) (l: (@list var_sub)) (t: term) (retval: Z) (retval_2: Z) (v: Z) (res_type: Z) ,
+  [| (retval <> 0) |] 
+  &&  [| (res_type = 0) |] 
+  &&  [| (v = 0) |] 
+  &&  [| (retval_2 <> 0) |] 
+  &&  [| (thm_pre <> 0) |] 
+  &&  [| (safeExec ATrue (thm_app_rel (t) (l) (g)) X ) |]
+  &&  ((&((retval_2)  # "solve_res" ->ₛ "type")) # Int  |-> res_type)
+  **  ((&((retval_2)  # "solve_res" ->ₛ "d" .ₛ "ans")) # Int  |-> v)
+  **  (sll_var_sub_list lis_pre l )
+  **  (store_sub_thm_res thm_pre retval t l )
+  **  (store_term goal_pre g )
+|--
+  [| (retval <> 0) |] 
+  &&  [| (retval <> 0) |] 
+  &&  [| (res_type = 0) |] 
+  &&  [| (v = 0) |] 
+  &&  [| (retval_2 <> 0) |] 
+  &&  [| (thm_pre <> 0) |] 
+  &&  [| (safeExec ATrue (thm_app_rel (t) (l) (g)) X ) |]
+  &&  (store_sub_thm_res thm_pre retval t l )
+  **  ((&((retval_2)  # "solve_res" ->ₛ "type")) # Int  |-> res_type)
+  **  ((&((retval_2)  # "solve_res" ->ₛ "d" .ₛ "ans")) # Int  |-> v)
+  **  (sll_var_sub_list lis_pre l )
+  **  (store_term goal_pre g )
+.
+
+Definition thm_apply_partial_solve_wit_4 := thm_apply_partial_solve_wit_4_pure -> thm_apply_partial_solve_wit_4_aux.
+
+Definition thm_apply_partial_solve_wit_5 := 
+forall (goal_pre: Z) (lis_pre: Z) (thm_pre: Z) (X: (solve_res -> (unit -> Prop))) (g: term) (l: (@list var_sub)) (t: term) (retval: Z) (retval_2: Z) (v: Z) (res_type: Z) (pq: partial_quant) (st: term) ,
+  [| (thm_subst_allres_rel t l pq st ) |] 
+  &&  [| (retval <> 0) |] 
+  &&  [| (res_type = 0) |] 
+  &&  [| (v = 0) |] 
+  &&  [| (retval_2 <> 0) |] 
+  &&  [| (thm_pre <> 0) |] 
+  &&  [| (safeExec ATrue (thm_app_rel (t) (l) (g)) X ) |]
+  &&  (store_partial_quant thm_pre retval pq )
+  **  (store_term retval st )
+  **  ((&((retval_2)  # "solve_res" ->ₛ "type")) # Int  |-> res_type)
+  **  ((&((retval_2)  # "solve_res" ->ₛ "d" .ₛ "ans")) # Int  |-> v)
+  **  (sll_var_sub_list lis_pre l )
+  **  (store_term goal_pre g )
+|--
+  [| (thm_subst_allres_rel t l pq st ) |] 
+  &&  [| (retval <> 0) |] 
+  &&  [| (res_type = 0) |] 
+  &&  [| (v = 0) |] 
+  &&  [| (retval_2 <> 0) |] 
+  &&  [| (thm_pre <> 0) |] 
+  &&  [| (safeExec ATrue (thm_app_rel (t) (l) (g)) X ) |]
+  &&  (store_term retval st )
+  **  (store_term goal_pre g )
+  **  (store_partial_quant thm_pre retval pq )
+  **  ((&((retval_2)  # "solve_res" ->ₛ "type")) # Int  |-> res_type)
+  **  ((&((retval_2)  # "solve_res" ->ₛ "d" .ₛ "ans")) # Int  |-> v)
+  **  (sll_var_sub_list lis_pre l )
+.
+
+Definition thm_apply_partial_solve_wit_6_pure := 
+forall (goal_pre: Z) (lis_pre: Z) (thm_pre: Z) (X: (solve_res -> (unit -> Prop))) (g: term) (l: (@list var_sub)) (t: term) (retval_2: Z) (retval_3: Z) (v: Z) (res_type: Z) (pq: partial_quant) (st: term) (retval: Z) ,
+  [| (retval = 0) |] 
+  &&  [| (retval = (term_alpha_eqn (st) (g))) |] 
+  &&  [| (thm_subst_allres_rel t l pq st ) |] 
+  &&  [| (retval_2 <> 0) |] 
+  &&  [| (res_type = 0) |] 
+  &&  [| (v = 0) |] 
+  &&  [| (retval_3 <> 0) |] 
+  &&  [| (thm_pre <> 0) |] 
+  &&  [| (safeExec ATrue (thm_app_rel (t) (l) (g)) X ) |]
+  &&  (store_term retval_2 st )
+  **  (store_term goal_pre g )
+  **  ((( &( "thm_ins" ) )) # Ptr  |-> retval_2)
+  **  ((( &( "thm" ) )) # Ptr  |-> thm_pre)
+  **  (store_partial_quant thm_pre retval_2 pq )
+  **  ((( &( "res" ) )) # Ptr  |-> retval_3)
+  **  ((&((retval_3)  # "solve_res" ->ₛ "type")) # Int  |-> 1)
+  **  ((&((retval_3)  # "solve_res" ->ₛ "d" .ₛ "ans")) # Int  |-> v)
+  **  (sll_var_sub_list lis_pre l )
+  **  ((( &( "goal" ) )) # Ptr  |-> goal_pre)
+  **  ((( &( "lis" ) )) # Ptr  |-> lis_pre)
+|--
+  [| (0 = 0) |]
+.
+
+Definition thm_apply_partial_solve_wit_6_aux := 
+forall (goal_pre: Z) (lis_pre: Z) (thm_pre: Z) (X: (solve_res -> (unit -> Prop))) (g: term) (l: (@list var_sub)) (t: term) (retval: Z) (retval_2: Z) (v: Z) (res_type: Z) (pq: partial_quant) (st: term) (retval_3: Z) ,
+  [| (retval_3 = 0) |] 
+  &&  [| (retval_3 = (term_alpha_eqn (st) (g))) |] 
+  &&  [| (thm_subst_allres_rel t l pq st ) |] 
+  &&  [| (retval <> 0) |] 
+  &&  [| (res_type = 0) |] 
+  &&  [| (v = 0) |] 
+  &&  [| (retval_2 <> 0) |] 
+  &&  [| (thm_pre <> 0) |] 
+  &&  [| (safeExec ATrue (thm_app_rel (t) (l) (g)) X ) |]
+  &&  (store_term retval st )
+  **  (store_term goal_pre g )
+  **  (store_partial_quant thm_pre retval pq )
+  **  ((&((retval_2)  # "solve_res" ->ₛ "type")) # Int  |-> 1)
+  **  ((&((retval_2)  # "solve_res" ->ₛ "d" .ₛ "ans")) # Int  |-> v)
+  **  (sll_var_sub_list lis_pre l )
+|--
+  [| (0 = 0) |] 
+  &&  [| (retval_3 = 0) |] 
+  &&  [| (retval_3 = (term_alpha_eqn (st) (g))) |] 
+  &&  [| (thm_subst_allres_rel t l pq st ) |] 
+  &&  [| (retval <> 0) |] 
+  &&  [| (res_type = 0) |] 
+  &&  [| (v = 0) |] 
+  &&  [| (retval_2 <> 0) |] 
+  &&  [| (thm_pre <> 0) |] 
+  &&  [| (safeExec ATrue (thm_app_rel (t) (l) (g)) X ) |]
+  &&  ((&((retval_2)  # "solve_res" ->ₛ "d" .ₛ "ans")) # Int  |-> 0)
+  **  (store_term retval st )
+  **  (store_term goal_pre g )
+  **  (store_partial_quant thm_pre retval pq )
+  **  ((&((retval_2)  # "solve_res" ->ₛ "type")) # Int  |-> 1)
+  **  (sll_var_sub_list lis_pre l )
+.
+
+Definition thm_apply_partial_solve_wit_6 := thm_apply_partial_solve_wit_6_pure -> thm_apply_partial_solve_wit_6_aux.
+
+Definition thm_apply_partial_solve_wit_7 := 
+forall (goal_pre: Z) (lis_pre: Z) (thm_pre: Z) (X: (solve_res -> (unit -> Prop))) (g: term) (l: (@list var_sub)) (t: term) (retval: Z) (retval_2: Z) (v: Z) (res_type: Z) (pq: partial_quant) (st: term) (retval_3: Z) (v_2: Z) ,
+  [| (v_2 = 0) |] 
+  &&  [| (retval_3 = 0) |] 
+  &&  [| (retval_3 = (term_alpha_eqn (st) (g))) |] 
+  &&  [| (thm_subst_allres_rel t l pq st ) |] 
+  &&  [| (retval <> 0) |] 
+  &&  [| (res_type = 0) |] 
+  &&  [| (v = 0) |] 
+  &&  [| (retval_2 <> 0) |] 
+  &&  [| (thm_pre <> 0) |] 
+  &&  [| (safeExec ATrue (thm_app_rel (t) (l) (g)) X ) |]
+  &&  ((&((retval_2)  # "solve_res" ->ₛ "d" .ₛ "list")) # Ptr  |-> v_2)
+  **  (store_term retval st )
+  **  (store_term goal_pre g )
+  **  (store_partial_quant thm_pre retval pq )
+  **  ((&((retval_2)  # "solve_res" ->ₛ "type")) # Int  |-> 1)
+  **  (sll_var_sub_list lis_pre l )
+|--
+  [| (v_2 = 0) |] 
+  &&  [| (retval_3 = 0) |] 
+  &&  [| (retval_3 = (term_alpha_eqn (st) (g))) |] 
+  &&  [| (thm_subst_allres_rel t l pq st ) |] 
+  &&  [| (retval <> 0) |] 
+  &&  [| (res_type = 0) |] 
+  &&  [| (v = 0) |] 
+  &&  [| (retval_2 <> 0) |] 
+  &&  [| (thm_pre <> 0) |] 
+  &&  [| (safeExec ATrue (thm_app_rel (t) (l) (g)) X ) |]
+  &&  (store_term retval st )
+  **  ((&((retval_2)  # "solve_res" ->ₛ "d" .ₛ "list")) # Ptr  |-> v_2)
+  **  (store_term goal_pre g )
+  **  (store_partial_quant thm_pre retval pq )
+  **  ((&((retval_2)  # "solve_res" ->ₛ "type")) # Int  |-> 1)
+  **  (sll_var_sub_list lis_pre l )
+.
+
+Definition thm_apply_partial_solve_wit_8_pure := 
+forall (goal_pre: Z) (lis_pre: Z) (thm_pre: Z) (X: (solve_res -> (unit -> Prop))) (g: term) (l: (@list var_sub)) (t: term) (retval_2: Z) (retval_3: Z) (v: Z) (res_type: Z) (pq: partial_quant) (st: term) (retval_4: Z) (v_2: Z) (retval: Z) ,
+  [| (retval <> 0) |] 
+  &&  [| (v_2 = 0) |] 
+  &&  [| (retval_4 = 0) |] 
+  &&  [| (retval_4 = (term_alpha_eqn (st) (g))) |] 
+  &&  [| (thm_subst_allres_rel t l pq st ) |] 
+  &&  [| (retval_2 <> 0) |] 
+  &&  [| (res_type = 0) |] 
+  &&  [| (v = 0) |] 
+  &&  [| (retval_3 <> 0) |] 
+  &&  [| (thm_pre <> 0) |] 
+  &&  [| (safeExec ATrue (thm_app_rel (t) (l) (g)) X ) |]
+  &&  (store_term retval_2 st )
+  **  (store_term retval st )
+  **  ((( &( "thm_ins_c" ) )) # Ptr  |-> retval)
+  **  ((( &( "res" ) )) # Ptr  |-> retval_3)
+  **  ((&((retval_3)  # "solve_res" ->ₛ "d" .ₛ "list")) # Ptr  |-> v_2)
+  **  (store_term goal_pre g )
+  **  ((( &( "thm_ins" ) )) # Ptr  |-> retval_2)
+  **  ((( &( "thm" ) )) # Ptr  |-> thm_pre)
+  **  (store_partial_quant thm_pre retval_2 pq )
+  **  ((&((retval_3)  # "solve_res" ->ₛ "type")) # Int  |-> 1)
+  **  (sll_var_sub_list lis_pre l )
+  **  ((( &( "goal" ) )) # Ptr  |-> goal_pre)
+  **  ((( &( "lis" ) )) # Ptr  |-> lis_pre)
+|--
+  [| ((term_alpha_eqn (st) (g)) = 0) |] 
+  &&  [| (thm_subst_allres_rel t l pq st ) |] 
+  &&  [| (safeExec ATrue (thm_app_rel (t) (l) (g)) X ) |]
+.
+
+Definition thm_apply_partial_solve_wit_8_aux := 
+forall (goal_pre: Z) (lis_pre: Z) (thm_pre: Z) (X: (solve_res -> (unit -> Prop))) (g: term) (l: (@list var_sub)) (t: term) (retval: Z) (retval_2: Z) (v: Z) (res_type: Z) (pq: partial_quant) (st: term) (retval_3: Z) (v_2: Z) (retval_4: Z) ,
+  [| (retval_4 <> 0) |] 
+  &&  [| (v_2 = 0) |] 
+  &&  [| (retval_3 = 0) |] 
+  &&  [| (retval_3 = (term_alpha_eqn (st) (g))) |] 
+  &&  [| (thm_subst_allres_rel t l pq st ) |] 
+  &&  [| (retval <> 0) |] 
+  &&  [| (res_type = 0) |] 
+  &&  [| (v = 0) |] 
+  &&  [| (retval_2 <> 0) |] 
+  &&  [| (thm_pre <> 0) |] 
+  &&  [| (safeExec ATrue (thm_app_rel (t) (l) (g)) X ) |]
+  &&  (store_term retval st )
+  **  (store_term retval_4 st )
+  **  ((&((retval_2)  # "solve_res" ->ₛ "d" .ₛ "list")) # Ptr  |-> v_2)
+  **  (store_term goal_pre g )
+  **  (store_partial_quant thm_pre retval pq )
+  **  ((&((retval_2)  # "solve_res" ->ₛ "type")) # Int  |-> 1)
+  **  (sll_var_sub_list lis_pre l )
+|--
+  [| ((term_alpha_eqn (st) (g)) = 0) |] 
+  &&  [| (thm_subst_allres_rel t l pq st ) |] 
+  &&  [| (safeExec ATrue (thm_app_rel (t) (l) (g)) X ) |] 
+  &&  [| (retval_4 <> 0) |] 
+  &&  [| (v_2 = 0) |] 
+  &&  [| (retval_3 = 0) |] 
+  &&  [| (retval_3 = (term_alpha_eqn (st) (g))) |] 
+  &&  [| (thm_subst_allres_rel t l pq st ) |] 
+  &&  [| (retval <> 0) |] 
+  &&  [| (res_type = 0) |] 
+  &&  [| (v = 0) |] 
+  &&  [| (retval_2 <> 0) |] 
+  &&  [| (thm_pre <> 0) |] 
+  &&  [| (safeExec ATrue (thm_app_rel (t) (l) (g)) X ) |]
+  &&  (store_term retval st )
+  **  (store_term retval_4 st )
+  **  ((&((retval_2)  # "solve_res" ->ₛ "d" .ₛ "list")) # Ptr  |-> v_2)
+  **  (store_term goal_pre g )
+  **  (store_partial_quant thm_pre retval pq )
+  **  ((&((retval_2)  # "solve_res" ->ₛ "type")) # Int  |-> 1)
+  **  (sll_var_sub_list lis_pre l )
+.
+
+Definition thm_apply_partial_solve_wit_8 := thm_apply_partial_solve_wit_8_pure -> thm_apply_partial_solve_wit_8_aux.
+
+Definition thm_apply_partial_solve_wit_9_pure := 
+forall (goal_pre: Z) (lis_pre: Z) (thm_pre: Z) (X: (solve_res -> (unit -> Prop))) (g: term) (l: (@list var_sub)) (t: term) (retval: Z) (retval_2: Z) (v: Z) (res_type: Z) (pq: partial_quant) (st: term) (retval_3: Z) (v_2: Z) (retval_4: Z) (R: ((term * (@list term)) -> (unit -> Prop))) ,
+  [| (safeExec ATrue (check_rel (st) (g)) R ) |] 
+  &&  [| (retval_4 <> 0) |] 
+  &&  [| (v_2 = 0) |] 
+  &&  [| (retval_3 = 0) |] 
+  &&  [| (retval_3 = (term_alpha_eqn (st) (g))) |] 
+  &&  [| (thm_subst_allres_rel t l pq st ) |] 
+  &&  [| (retval <> 0) |] 
+  &&  [| (res_type = 0) |] 
+  &&  [| (v = 0) |] 
+  &&  [| (retval_2 <> 0) |] 
+  &&  [| (thm_pre <> 0) |] 
+  &&  [| (safeExec ATrue (thm_app_rel (t) (l) (g)) X ) |]
+  &&  (store_term retval st )
+  **  (store_term retval_4 st )
+  **  ((( &( "thm_ins_c" ) )) # Ptr  |-> retval_4)
+  **  ((( &( "res" ) )) # Ptr  |-> retval_2)
+  **  ((&((retval_2)  # "solve_res" ->ₛ "d" .ₛ "list")) # Ptr  |-> v_2)
+  **  (store_term goal_pre g )
+  **  ((( &( "thm_ins" ) )) # Ptr  |-> retval)
+  **  ((( &( "thm" ) )) # Ptr  |-> thm_pre)
+  **  (store_partial_quant thm_pre retval pq )
+  **  ((&((retval_2)  # "solve_res" ->ₛ "type")) # Int  |-> 1)
+  **  (sll_var_sub_list lis_pre l )
+  **  ((( &( "goal" ) )) # Ptr  |-> goal_pre)
+  **  ((( &( "lis" ) )) # Ptr  |-> lis_pre)
+|--
+  [| (safeExec ATrue (check_rel (st) (g)) R ) |]
+.
+
+Definition thm_apply_partial_solve_wit_9_aux := 
+forall (goal_pre: Z) (lis_pre: Z) (thm_pre: Z) (X: (solve_res -> (unit -> Prop))) (g: term) (l: (@list var_sub)) (t: term) (retval: Z) (retval_2: Z) (v: Z) (res_type: Z) (pq: partial_quant) (st: term) (retval_3: Z) (v_2: Z) (retval_4: Z) (R: ((term * (@list term)) -> (unit -> Prop))) ,
+  [| (safeExec ATrue (check_rel (st) (g)) R ) |] 
+  &&  [| (retval_4 <> 0) |] 
+  &&  [| (v_2 = 0) |] 
+  &&  [| (retval_3 = 0) |] 
+  &&  [| (retval_3 = (term_alpha_eqn (st) (g))) |] 
+  &&  [| (thm_subst_allres_rel t l pq st ) |] 
+  &&  [| (retval <> 0) |] 
+  &&  [| (res_type = 0) |] 
+  &&  [| (v = 0) |] 
+  &&  [| (retval_2 <> 0) |] 
+  &&  [| (thm_pre <> 0) |] 
+  &&  [| (safeExec ATrue (thm_app_rel (t) (l) (g)) X ) |]
+  &&  (store_term retval st )
+  **  (store_term retval_4 st )
+  **  ((&((retval_2)  # "solve_res" ->ₛ "d" .ₛ "list")) # Ptr  |-> v_2)
+  **  (store_term goal_pre g )
+  **  (store_partial_quant thm_pre retval pq )
+  **  ((&((retval_2)  # "solve_res" ->ₛ "type")) # Int  |-> 1)
+  **  (sll_var_sub_list lis_pre l )
+|--
+  [| (safeExec ATrue (check_rel (st) (g)) R ) |] 
+  &&  [| (safeExec ATrue (check_rel (st) (g)) R ) |] 
+  &&  [| (retval_4 <> 0) |] 
+  &&  [| (v_2 = 0) |] 
+  &&  [| (retval_3 = 0) |] 
+  &&  [| (retval_3 = (term_alpha_eqn (st) (g))) |] 
+  &&  [| (thm_subst_allres_rel t l pq st ) |] 
+  &&  [| (retval <> 0) |] 
+  &&  [| (res_type = 0) |] 
+  &&  [| (v = 0) |] 
+  &&  [| (retval_2 <> 0) |] 
+  &&  [| (thm_pre <> 0) |] 
+  &&  [| (safeExec ATrue (thm_app_rel (t) (l) (g)) X ) |]
+  &&  (store_term retval_4 st )
+  **  (store_term goal_pre g )
+  **  (store_term retval st )
+  **  ((&((retval_2)  # "solve_res" ->ₛ "d" .ₛ "list")) # Ptr  |-> v_2)
+  **  (store_partial_quant thm_pre retval pq )
+  **  ((&((retval_2)  # "solve_res" ->ₛ "type")) # Int  |-> 1)
+  **  (sll_var_sub_list lis_pre l )
+.
+
+Definition thm_apply_partial_solve_wit_9 := thm_apply_partial_solve_wit_9_pure -> thm_apply_partial_solve_wit_9_aux.
+
+Definition thm_apply_which_implies_wit_1 := 
+forall (res: Z) ,
+  (store_solve_res res (SRBool (0)) )
+|--
+  EX (v: Z)  (res_type: Z) ,
+  [| (res_type = 0) |] 
+  &&  [| (v = 0) |]
+  &&  ((&((res)  # "solve_res" ->ₛ "type")) # Int  |-> res_type)
+  **  ((&((res)  # "solve_res" ->ₛ "d" .ₛ "ans")) # Int  |-> v)
+.
+
+Definition thm_apply_which_implies_wit_2 := 
+forall (l: (@list var_sub)) (t: term) (thm_ins: Z) (thm: Z) ,
+  [| (thm_ins <> 0) |]
+  &&  (store_sub_thm_res thm thm_ins t l )
+|--
+  EX (pq: partial_quant)  (st: term) ,
+  [| (thm_subst_allres_rel t l pq st ) |]
+  &&  (store_partial_quant thm thm_ins pq )
+  **  (store_term thm_ins st )
+.
+
+Definition thm_apply_which_implies_wit_3 := 
+forall (res: Z) (v_2: Z) ,
+  [| (v_2 = 0) |]
+  &&  ((&((res)  # "solve_res" ->ₛ "d" .ₛ "ans")) # Int  |-> v_2)
+|--
+  EX (v: Z) ,
+  [| (v = 0) |]
+  &&  ((&((res)  # "solve_res" ->ₛ "d" .ₛ "list")) # Ptr  |-> v)
+.
+
+Definition thm_apply_which_implies_wit_4 := 
+forall (X: (solve_res -> (unit -> Prop))) (g: term) (l: (@list var_sub)) (t: term) (st: term) (pq: partial_quant) ,
+  [| ((term_alpha_eqn (st) (g)) = 0) |] 
+  &&  [| (thm_subst_allres_rel t l pq st ) |] 
+  &&  [| (safeExec ATrue (thm_app_rel (t) (l) (g)) X ) |]
+  &&  emp
+|--
+  EX (R: ((term * (@list term)) -> (unit -> Prop))) ,
+  [| (safeExec ATrue (check_rel (st) (g)) R ) |]
+  &&  emp
+.
+
 Module Type VC_Correct.
 
 Axiom proof_of_sub_thm_safety_wit_1 : sub_thm_safety_wit_1.
@@ -1554,5 +2216,31 @@ Axiom proof_of_check_list_gen_which_implies_wit_1 : check_list_gen_which_implies
 Axiom proof_of_check_list_gen_which_implies_wit_2 : check_list_gen_which_implies_wit_2.
 Axiom proof_of_check_list_gen_which_implies_wit_3 : check_list_gen_which_implies_wit_3.
 Axiom proof_of_check_list_gen_which_implies_wit_4 : check_list_gen_which_implies_wit_4.
+Axiom proof_of_thm_apply_safety_wit_1 : thm_apply_safety_wit_1.
+Axiom proof_of_thm_apply_safety_wit_2 : thm_apply_safety_wit_2.
+Axiom proof_of_thm_apply_safety_wit_3 : thm_apply_safety_wit_3.
+Axiom proof_of_thm_apply_safety_wit_4 : thm_apply_safety_wit_4.
+Axiom proof_of_thm_apply_safety_wit_5 : thm_apply_safety_wit_5.
+Axiom proof_of_thm_apply_safety_wit_6 : thm_apply_safety_wit_6.
+Axiom proof_of_thm_apply_return_wit_1_1 : thm_apply_return_wit_1_1.
+Axiom proof_of_thm_apply_return_wit_1_2 : thm_apply_return_wit_1_2.
+Axiom proof_of_thm_apply_return_wit_1_3 : thm_apply_return_wit_1_3.
+Axiom proof_of_thm_apply_partial_solve_wit_1 : thm_apply_partial_solve_wit_1.
+Axiom proof_of_thm_apply_partial_solve_wit_2 : thm_apply_partial_solve_wit_2.
+Axiom proof_of_thm_apply_partial_solve_wit_3 : thm_apply_partial_solve_wit_3.
+Axiom proof_of_thm_apply_partial_solve_wit_4_pure : thm_apply_partial_solve_wit_4_pure.
+Axiom proof_of_thm_apply_partial_solve_wit_4 : thm_apply_partial_solve_wit_4.
+Axiom proof_of_thm_apply_partial_solve_wit_5 : thm_apply_partial_solve_wit_5.
+Axiom proof_of_thm_apply_partial_solve_wit_6_pure : thm_apply_partial_solve_wit_6_pure.
+Axiom proof_of_thm_apply_partial_solve_wit_6 : thm_apply_partial_solve_wit_6.
+Axiom proof_of_thm_apply_partial_solve_wit_7 : thm_apply_partial_solve_wit_7.
+Axiom proof_of_thm_apply_partial_solve_wit_8_pure : thm_apply_partial_solve_wit_8_pure.
+Axiom proof_of_thm_apply_partial_solve_wit_8 : thm_apply_partial_solve_wit_8.
+Axiom proof_of_thm_apply_partial_solve_wit_9_pure : thm_apply_partial_solve_wit_9_pure.
+Axiom proof_of_thm_apply_partial_solve_wit_9 : thm_apply_partial_solve_wit_9.
+Axiom proof_of_thm_apply_which_implies_wit_1 : thm_apply_which_implies_wit_1.
+Axiom proof_of_thm_apply_which_implies_wit_2 : thm_apply_which_implies_wit_2.
+Axiom proof_of_thm_apply_which_implies_wit_3 : thm_apply_which_implies_wit_3.
+Axiom proof_of_thm_apply_which_implies_wit_4 : thm_apply_which_implies_wit_4.
 
 End VC_Correct.
