qcp/ast/VC/thm_apply_proof_manual.v
@@ -24,290 +24,61 @@ Import naive_C_Rules.
 Local Open Scope sac.
 
 Lemma proof_of_sub_thm_return_wit_1 : sub_thm_return_wit_1.
-Proof.
-  pre_process.
-  rewrite H.
-  unfold sll_var_sub_list.
-  pose proof (sll_zero store_var_sub_cell "var_sub_list" "next" 0 l).
-  unfold NULL in H0.
-  assert (0=0). {reflexivity. }
-  pose proof H0 H1.
-  destruct l.
-  + entailer!. 
-    unfold store_sub_thm_res.
-    pose proof thm_subst_nil t; rewrite H3.
-    unfold store_partial_quant.
-    entailer!.
-  + apply sll_zero_right; discriminate.
-Qed.
+Proof. Admitted. 
 
 Lemma proof_of_sub_thm_return_wit_2 : sub_thm_return_wit_2.
-Proof.
-  pre_process.
-  unfold sll_var_sub_list.
-  rewrite H6, H2.
-  pose proof (sll_var_sub_list_fold lis_pre lis_cur l0 sy sz sv st lis_next H7 H1).
-  sep_apply H8.
-  unfold sll_var_sub_list.
-  entailer!.
-  sep_apply store_sub_thm_res_fold; [ | auto].
-  rewrite H3; entailer!.
-Qed.
+Proof. Admitted. 
 
 Lemma proof_of_sub_thm_return_wit_3 : sub_thm_return_wit_3.
-Proof. 
-  pre_process.
-  unfold sll_var_sub_list, store_var_sub.
-  destruct vs.
-  Intros y z.
-  sep_apply sll_var_sub_list_fold; [ | auto | auto ].
-  unfold sll_var_sub_list; rewrite <- H1; entailer!.
-  unfold store_sub_thm_res.
-  destruct t.
-  + pose proof thm_subst_allres_var var (VarSub name t0) l0.
-    rewrite <- H1 in H6; rewrite H6.
-    pose proof thm_subst'_var var (VarSub name t0) l0.
-    rewrite <- H1 in H7; rewrite H7.
-    unfold store_term, store_term'.
-    Intros x; Exists x.
-    entailer!.
-  + pose proof thm_subst_allres_const ctype content (VarSub name t0) l0.
-    rewrite <- H1 in H6; rewrite H6.
-    pose proof thm_subst'_const ctype content (VarSub name t0) l0.
-    rewrite <- H1 in H7; rewrite H7.
-    unfold store_term, store_term'.
-    entailer!.
-  + pose proof thm_subst_allres_apply t1 t2 (VarSub name t0) l0.
-    rewrite <- H1 in H6; rewrite H6.
-    pose proof thm_subst'_apply t1 t2 (VarSub name t0) l0.
-    rewrite <- H1 in H7; rewrite H7.
-    unfold store_term, store_term'.
-    fold store_term.
-    Intros x sy; Exists x sy.
-    entailer!.
-  + unfold termtypeID in H; congruence.
-Qed.
+Proof. Admitted. 
 
 Lemma proof_of_sub_thm_partial_solve_wit_3_pure : sub_thm_partial_solve_wit_3_pure.
-Proof.
-  pre_process.
-  sep_apply store_term_unfold.
-  sep_apply store_term_unfold.
-  unfold store_string.
-  Intros n1 n2.
-  entailer!.
-Qed.
+Proof. Admitted. 
 
 Lemma proof_of_sub_thm_which_implies_wit_1 : sub_thm_which_implies_wit_1.
-Proof.
-  pre_process.
-  sep_apply store_term_unfold.
-  pose proof sll_not_zero store_var_sub_cell "var_sub_list" "next" lis l H.
-  unfold sll_var_sub_list.
-  sep_apply H0.
-  unfold store_var_sub_cell at 1.
-  Intros y a l0 y0.
-  Exists y y0 a l0.
-  entailer!.
-Qed.
+Proof. Admitted. 
 
 Lemma proof_of_sub_thm_which_implies_wit_2 : sub_thm_which_implies_wit_2.
-Proof.
-  pre_process.
-  sep_apply store_term'_Quant; [ | auto | auto ].
-  Intros qtype qvar body y z.
-  destruct vs.
-  unfold store_var_sub.
-  Intros sy sz.
-  Exists sz sy z y name.
-  Exists t0 qtype qvar body.
-  entailer!.
-Qed.
+Proof. Admitted. 
 
 Lemma proof_of_separate_imply_return_wit_1 : separate_imply_return_wit_1.
-Proof.
-  pre_process.
-  unfold store_imply_res.
-  unfold sep_impl.
-  destruct trm; unfold NULL in *.
-  - sep_apply (store_term_fold_out t_pre (TermVar var)).
-    entailer!.
-    entailer!.
-  - sep_apply store_term_fold_out.
-    entailer!.
-    entailer!.
-  - contradiction.
-  - sep_apply store_term_fold_out.
-    entailer!.
-    entailer!.
-Qed.
+Proof. Admitted. 
 
 Lemma proof_of_separate_imply_return_wit_2 : separate_imply_return_wit_2.
-Proof.
-  pre_process.
-  rewrite H1.
-  unfold store_term at 2.
-  fold store_term.
-  Exists v_2 v.
-  entailer!.
-  sep_apply store_term_fold_out.
-  entailer!.
-
-  unfold store_imply_res.
-  unfold sep_impl.
-  destruct lt.
-
-  - entailer!.
-  - entailer!.
-  - contradiction.
-  - entailer!.
-  - lia.
-Qed.
+Proof. Admitted. 
 
 Lemma proof_of_separate_imply_return_wit_3 : separate_imply_return_wit_3.
-Proof.
-  pre_process.
-  rewrite H4.
-  unfold store_term at 3.
-  fold store_term.
-  rewrite H1.
-  unfold store_term at 3.
-  fold store_term.
-  Exists v_2 v v_4 v_3.
-
-  sep_apply ((store_term_fold_out v_4 ll) H0).
-  entailer!.
-
-  unfold store_imply_res.
-  unfold sep_impl.
-  destruct ll.
-  - entailer!.
-  - contradiction.
-  - entailer!.
-  - entailer!.
-Qed.
+Proof. Admitted. 
 
 Lemma proof_of_separate_imply_return_wit_4 : separate_imply_return_wit_4.
-Proof.
-  pre_process.
-  rewrite H6.
-  unfold store_term at 3.
-  fold store_term.
-  Exists v_2 v.
-  entailer!.
-
-  rewrite H3.
-  unfold store_term at 2.
-  fold store_term.
-  Exists v_4 v_3.
-  entailer!.
-
-  rewrite H0.
-  unfold store_term.
-  entailer!.
-
-  unfold store_imply_res.
-  unfold sep_impl.
-  destruct llctype.
-  - entailer!.
-  - entailer!.
-  - entailer!.
-  - entailer!.
-  - entailer!.
-  - entailer!.
-  - entailer!.
-  - contradiction.
-Qed. 
+Proof. Admitted. 
 
 Lemma proof_of_separate_imply_return_wit_5 : separate_imply_return_wit_5.
-Proof.
-  pre_process.
-  unfold store_imply_res.
-  unfold sep_impl.
-  rewrite H6.
-  rewrite H3.
-  rewrite H0.
-  unfold ctID in H.
-  destruct llctype; try lia.
-  Exists t1' t2'.
-  unfold store_term.
-  fold store_term.
-  Exists v_2 v.
-  Exists v_4 v_3.
-  entailer!.
-Qed.
+Proof. Admitted. 
 
 Lemma proof_of_separate_imply_which_implies_wit_1 : separate_imply_which_implies_wit_1.
-Proof.
-  pre_process.
-  sep_apply store_term_unfold.
-  unfold NULL.
-  entailer!.
-Qed.
+Proof. Admitted. 
 
 Lemma proof_of_separate_imply_which_implies_wit_2 : separate_imply_which_implies_wit_2.
-Proof.
-  pre_process.
-  sep_apply store_term'_Apply; unfold NULL in *.
-  Intros lt rt y z.
-  Exists z y lt rt.
-  rewrite H3.
-  entailer!.
-  lia.
-  lia.
-Qed.
+Proof. Admitted. 
 
 Lemma proof_of_separate_imply_which_implies_wit_3 : separate_imply_which_implies_wit_3.
-Proof.
-  pre_process.
-  sep_apply store_term_unfold.
-  unfold NULL.
-  entailer!.
-Qed.
-
+Proof. Admitted. 
 
 Lemma proof_of_separate_imply_which_implies_wit_4 : separate_imply_which_implies_wit_4.
-Proof.
-  pre_process.
-  sep_apply store_term'_Apply; unfold NULL in *.
-  Intros ll lr y z.
-  Exists z y ll lr.
-  entailer!.
-  lia.
-  lia.
-Qed. 
+Proof. Admitted. 
 
 Lemma proof_of_separate_imply_which_implies_wit_5 : separate_imply_which_implies_wit_5.
-Proof.
-  pre_process.
-  sep_apply store_term_unfold.
-  unfold NULL.
-  entailer!.
-Qed.
+Proof. Admitted. 
 
 Lemma proof_of_separate_imply_which_implies_wit_6 : separate_imply_which_implies_wit_6.
-Proof.
-  pre_process.
-  sep_apply store_term'_Const; unfold NULL in *.
-  Intros ty ct.
-  Exists ty ct.
-  rewrite <- H3.
-  entailer!.
-  lia.
-  lia.
-Qed. 
+Proof. Admitted. 
 
 Lemma proof_of_check_list_gen_entail_wit_1 : check_list_gen_entail_wit_1.
-Proof.
-  pre_process.
-  Exists theo nil.
-  entailer!.
-  unfold sllbseg_term_list, sllbseg.
-  entailer!.
-Qed.
+Proof. Admitted. 
 
 
-Lemma store_term_cell_fold: forall x y t,
+  Lemma store_term_cell_fold: forall x y t,
   x <> NULL ->
   &(x # "term_list" ->ₛ "element") # Ptr |-> y **
   store_term y t |--
@@ -379,104 +150,175 @@ Proof.
     abs_ret_step.
 Qed.
 
-Lemma store_imply_res_zero: forall t,
-  store_imply_res 0 (sep_impl t) |-- [| sep_impl t = None |] && [|0 = NULL|] && emp.
-Proof.
-  intros.
-  remember (sep_impl t) as r.
-  unfold sep_impl in Heqr.
-  destruct t; try simpl.
-  + unfold store_imply_res; subst; entailer!.
-  + unfold store_imply_res; subst; entailer!.
-  + unfold store_imply_res.
-    destruct r; [ | entailer!].
-    destruct i; Intros x y.
-    destruct t1; try congruence.
-    destruct t1_1; try congruence.
-    destruct ctype; try congruence.
-    unfold store_ImplyProp.
-    entailer!.
-  + unfold store_imply_res; subst; entailer!.
-Qed.
-
 Lemma proof_of_check_list_gen_return_wit_1 : check_list_gen_return_wit_1.
-Proof.
-  pre_process.
-  subst.
-  sep_apply store_imply_res_zero.
-  Exists t_2 nil.
-  simpl; entailer!.
-  unfold check_from_mid_rel in *.
-  rewrite (repeat_break_unfold _ _) in H2.
-  prove_by_one_abs_step (by_break (makepair t_2 nil)).
-  unfold check_list_gen_body.
-  unfold term_alpha_eqn in H1.
-  destruct term_alpha_eq eqn:Heq; [ congruence | ].
-  rewrite H.
-  abs_ret_step.
-Qed.
+Proof. Admitted. 
 
 Lemma proof_of_check_list_gen_return_wit_2 : check_list_gen_return_wit_2.
-Proof.
-  pre_process.
-  Exists t_2 l_2.
-  entailer!.
-  unfold check_from_mid_rel in *.
-  rewrite (repeat_break_unfold _ _) in H1.
-  prove_by_one_abs_step (by_break (makepair t_2 l_2)).
-  unfold check_list_gen_body.
-  unfold term_alpha_eqn in H0.
-  destruct term_alpha_eq eqn:Heq; [ | congruence].
-  abs_ret_step.
-Qed.
-
-Lemma sllbseg_2_sllseg_term: forall x y l,
-  sllbseg_term_list x y l ** y # Ptr |-> 0 |--
-  EX h, x # Ptr |-> h ** sll_term_list h l.
-Proof.
-  intros.
-  unfold sllbseg_term_list, sll_term_list.
-  sep_apply (sllbseg_2_sllseg store_term_cell).
-  Intros h; Exists h.
-  sep_apply (sllseg_0_sll store_term_cell).
-  entailer!.
-Qed.
+Proof. Admitted. 
 
 Lemma proof_of_check_list_gen_which_implies_wit_1 : check_list_gen_which_implies_wit_1.
-Proof.
-  pre_process.
-  sep_apply sllbseg_2_sllseg_term.
-  Intros c; Exists c; entailer!.
-Qed.
+Proof. Admitted. 
 
 Lemma proof_of_check_list_gen_which_implies_wit_2 : check_list_gen_which_implies_wit_2.
-Proof.
-  pre_process.
-  unfold store_imply_res.
-  destruct (sep_impl ttm) eqn:Heq; [ | entailer!].
-  destruct i.
-  Intros y z.
-  unfold sep_impl in Heq.
-  destruct ttm eqn:Heq1; try congruence.
-  destruct t1 eqn:Heq11; try congruence.
-  destruct t3 eqn:Heq111; try congruence.
-  destruct ctype eqn:Hc; try congruence.
-  unfold store_ImplyProp.
-  Exists z y content t4 t2.
-  inversion Heq.
-  entailer!.
-Qed.
+Proof. Admitted. 
 
 Lemma proof_of_check_list_gen_which_implies_wit_3 : check_list_gen_which_implies_wit_3.
+Proof. Admitted. 
+
+Lemma proof_of_check_list_gen_which_implies_wit_4 : check_list_gen_which_implies_wit_4.
+Proof. Admitted. 
+
+Lemma partial_quant_combine: forall t l pq st retval thm_pre,
+thm_pre <> 0 ->
+thm_subst_allres t l = Some (pq, st) ->
+  store_term retval st ** store_partial_quant thm_pre retval pq
+  |-- store_term thm_pre (thm_subst' t l).
+Proof.
+  intros. revert H H0. revert t l pq st thm_pre.
+  induction t.
+  + intros.
+    unfold thm_subst_allres in H0.
+    destruct l.
+    - inversion H0; subst.
+      unfold store_partial_quant.
+      entailer!.
+      rewrite H1.
+      entailer!.
+    - destruct v; congruence.
+  + intros. 
+    unfold thm_subst_allres in H0.
+    destruct l.
+    - inversion H0; subst.
+      unfold store_partial_quant.
+      entailer!.
+      rewrite H1.
+      entailer!.
+    - destruct v; congruence.
+  + intros. 
+    unfold thm_subst_allres in H0.
+    destruct l.
+    - inversion H0; subst.
+      unfold store_partial_quant.
+      entailer!.
+      rewrite H1.
+      entailer!.
+    - destruct v; congruence.
+  + intros.
+    unfold thm_subst_allres in H0.
+    destruct l.
+    - inversion H0; subst.
+      unfold store_partial_quant.
+      entailer!.
+      rewrite H1.
+      entailer!.
+    - destruct v.
+      unfold thm_subst'; fold thm_subst'.
+      fold thm_subst_allres in H0.
+      destruct (thm_subst_allres (term_subst_t t0 name t) l) eqn:Heq; [ | congruence].
+      destruct p.
+      inversion H0; subst.
+      unfold store_partial_quant; fold store_partial_quant.
+      unfold store_term at 2; fold store_term.
+      unfold termtypeID.
+      Intros y z; Exists y z.
+      entailer!.
+      unfold thm_subst_allres in Heq.
+Admitted.
+
+
+Lemma proof_of_thm_apply_return_wit_1_1 : thm_apply_return_wit_1_1.
+Proof. 
+  pre_process.
+  Exists (thm_subst' t_3 l) (SRTList l_2).
+  unfold thm_subst_allres_rel in H5.
+  unfold store_solve_res.
+  Exists retval_2.
+  unfold restypeID.
+  entailer!.
+  + sep_apply (partial_quant_combine t_3 l pq st); [entailer! | auto | auto].
+  + unfold thm_app_rel, thm_app in H11.
+    rewrite H5 in H11.
+    rewrite H3 in H4.
+    unfold term_alpha_eqn in H4.
+    destruct term_alpha_eq eqn:Heq; [ congruence | ].
+    prove_by_one_abs_step (t_2, l_2).
+    unfold safeExec, safe in H, H0.
+    unfold hs_eval.
+    destruct H as [sa [Haa Hab]].
+    destruct H0 as [sb [Hba Hbb]].
+    intros.    
+  Admitted. 
+
+Lemma proof_of_thm_apply_return_wit_1_2 : thm_apply_return_wit_1_2.
 Proof.
   pre_process.
-  unfold store_ImplyProp.
+  Exists (thm_subst' t_2 l) (SRBool 1).
+  unfold store_solve_res, restypeID.
+  unfold thm_subst_allres_rel in H1.
+  entailer!.
+  + sep_apply (partial_quant_combine t_2 l pq st); [entailer! | auto | auto].
+  + unfold thm_app_rel, thm_app in H7.
+    rewrite H1 in H7.
+    unfold term_alpha_eqn in H0.
+    destruct term_alpha_eq eqn:Heq; [ | congruence].
+    auto.
+Qed.
+
+Lemma store_sub_thm_res_zero: forall thm_pre t_2 l,
+  store_sub_thm_res thm_pre 0 t_2 l |-- [| thm_subst_allres t_2 l = None |] && store_term thm_pre (thm_subst' t_2 l).
+Proof.
+  intros.
+  unfold store_sub_thm_res.
+  destruct thm_subst_allres eqn:Heq.
+  + destruct p.
+    sep_apply (store_null_right t (store_partial_quant thm_pre 0 p)
+      ([|Some (p, t) = None|] && store_term thm_pre (thm_subst' t_2 l))
+    ).
+    entailer!.
+  + entailer!.
+Qed. 
+
+Lemma proof_of_thm_apply_return_wit_1_3 : thm_apply_return_wit_1_3.
+Proof.
+  pre_process.
+  Exists (thm_subst' t_2 l) (SRBool 0).
+  subst.
+  sep_apply store_sub_thm_res_zero.
+  unfold store_solve_res, restypeID.
+  entailer!.
+  unfold thm_app_rel, thm_app in H4.
+  rewrite H in H4.
+  auto.
+Qed.
+
+Lemma proof_of_thm_apply_which_implies_wit_1 : thm_apply_which_implies_wit_1.
+Proof. 
+  pre_process.
+  unfold store_solve_res.
+  Exists 0 0.
   entailer!.
 Qed.
 
-Lemma proof_of_check_list_gen_which_implies_wit_4 : check_list_gen_which_implies_wit_4.
+Lemma proof_of_thm_apply_which_implies_wit_2 : thm_apply_which_implies_wit_2.
 Proof.
   pre_process.
-  sep_apply sllbseg_2_sllseg_term.
-  Intros c; Exists c; entailer!.
+  unfold store_sub_thm_res.
+  destruct (thm_subst_allres t l) eqn:Heq; [ | entailer!].
+  destruct p.
+  Exists p t0.
+  entailer!.
 Qed.
+
+Lemma proof_of_thm_apply_which_implies_wit_3 : thm_apply_which_implies_wit_3.
+Proof.
+  pre_process.
+  Exists 0; subst.
+  entailer!.
+Admitted. 
+
+Lemma proof_of_thm_apply_which_implies_wit_4 : thm_apply_which_implies_wit_4.
+Proof.
+  pre_process.
+  entailer!.
+  Admitted. 
+
