qcp/ast/VC/thm_apply_proof_manual_c.v
@@ -1,0 +1,482 @@
+Require Import Coq.ZArith.ZArith.
+Require Import Coq.Bool.Bool.
+Require Import Coq.Strings.String.
+Require Import Coq.Lists.List.
+Require Import Coq.Classes.RelationClasses.
+Require Import Coq.Classes.Morphisms.
+Require Import Coq.micromega.Psatz.
+Require Import Coq.Sorting.Permutation.
+From AUXLib Require Import int_auto Axioms Feq Idents List_lemma VMap.
+Require Import SetsClass.SetsClass. Import SetsNotation.
+From SimpleC.SL Require Import Mem SeparationLogic.
+Require Import thm_apply_goal.
+Require Import Logic.LogicGenerator.demo932.Interface.
+Local Open Scope Z_scope.
+Local Open Scope sets.
+Local Open Scope string.
+Local Open Scope list.
+From MonadLib.StateRelMonad Require Import StateRelMonad StateRelBasic StateRelHoare FixpointLib safeexec_lib.
+Import naive_C_Rules.
+From SimpleC.EE Require Import ast_lib.
+From SimpleC.EE Require Import malloc.
+From SimpleC.EE Require Import sll_tmpl.
+Import naive_C_Rules.
+Local Open Scope sac.
+
+Lemma proof_of_sub_thm_return_wit_1 : sub_thm_return_wit_1.
+Proof.
+  pre_process.
+  rewrite H.
+  unfold sll_var_sub_list.
+  pose proof (sll_zero store_var_sub_cell "var_sub_list" "next" 0 l).
+  unfold NULL in H0.
+  assert (0=0). {reflexivity. }
+  pose proof H0 H1.
+  destruct l.
+  + entailer!. 
+    unfold store_sub_thm_res.
+    pose proof thm_subst_nil t; rewrite H3.
+    unfold store_partial_quant.
+    entailer!.
+  + apply sll_zero_right; discriminate.
+Qed.
+
+Lemma proof_of_sub_thm_return_wit_2 : sub_thm_return_wit_2.
+Proof.
+  pre_process.
+  unfold sll_var_sub_list.
+  rewrite H6, H2.
+  pose proof (sll_var_sub_list_fold lis_pre lis_cur l0 sy sz sv st lis_next H7 H1).
+  sep_apply H8.
+  unfold sll_var_sub_list.
+  entailer!.
+  sep_apply store_sub_thm_res_fold; [ | auto].
+  rewrite H3; entailer!.
+Qed.
+
+Lemma proof_of_sub_thm_return_wit_3 : sub_thm_return_wit_3.
+Proof. 
+  pre_process.
+  unfold sll_var_sub_list, store_var_sub.
+  destruct vs.
+  Intros y z.
+  sep_apply sll_var_sub_list_fold; [ | auto | auto ].
+  unfold sll_var_sub_list; rewrite <- H1; entailer!.
+  unfold store_sub_thm_res.
+  destruct t.
+  + pose proof thm_subst_allres_var var (VarSub name t0) l0.
+    rewrite <- H1 in H6; rewrite H6.
+    pose proof thm_subst'_var var (VarSub name t0) l0.
+    rewrite <- H1 in H7; rewrite H7.
+    unfold store_term, store_term'.
+    Intros x; Exists x.
+    entailer!.
+  + pose proof thm_subst_allres_const ctype content (VarSub name t0) l0.
+    rewrite <- H1 in H6; rewrite H6.
+    pose proof thm_subst'_const ctype content (VarSub name t0) l0.
+    rewrite <- H1 in H7; rewrite H7.
+    unfold store_term, store_term'.
+    entailer!.
+  + pose proof thm_subst_allres_apply t1 t2 (VarSub name t0) l0.
+    rewrite <- H1 in H6; rewrite H6.
+    pose proof thm_subst'_apply t1 t2 (VarSub name t0) l0.
+    rewrite <- H1 in H7; rewrite H7.
+    unfold store_term, store_term'.
+    fold store_term.
+    Intros x sy; Exists x sy.
+    entailer!.
+  + unfold termtypeID in H; congruence.
+Qed.
+
+Lemma proof_of_sub_thm_partial_solve_wit_3_pure : sub_thm_partial_solve_wit_3_pure.
+Proof.
+  pre_process.
+  sep_apply store_term_unfold.
+  sep_apply store_term_unfold.
+  unfold store_string.
+  Intros n1 n2.
+  entailer!.
+Qed.
+
+Lemma proof_of_sub_thm_which_implies_wit_1 : sub_thm_which_implies_wit_1.
+Proof.
+  pre_process.
+  sep_apply store_term_unfold.
+  pose proof sll_not_zero store_var_sub_cell "var_sub_list" "next" lis l H.
+  unfold sll_var_sub_list.
+  sep_apply H0.
+  unfold store_var_sub_cell at 1.
+  Intros y a l0 y0.
+  Exists y y0 a l0.
+  entailer!.
+Qed.
+
+Lemma proof_of_sub_thm_which_implies_wit_2 : sub_thm_which_implies_wit_2.
+Proof.
+  pre_process.
+  sep_apply store_term'_Quant; [ | auto | auto ].
+  Intros qtype qvar body y z.
+  destruct vs.
+  unfold store_var_sub.
+  Intros sy sz.
+  Exists sz sy z y name.
+  Exists t0 qtype qvar body.
+  entailer!.
+Qed.
+
+Lemma proof_of_separate_imply_return_wit_1 : separate_imply_return_wit_1.
+Proof.
+  pre_process.
+  unfold store_imply_res.
+  unfold sep_impl.
+  destruct trm; unfold NULL in *.
+  - sep_apply (store_term_fold_out t_pre (TermVar var)).
+    entailer!.
+    entailer!.
+  - sep_apply store_term_fold_out.
+    entailer!.
+    entailer!.
+  - contradiction.
+  - sep_apply store_term_fold_out.
+    entailer!.
+    entailer!.
+Qed.
+
+Lemma proof_of_separate_imply_return_wit_2 : separate_imply_return_wit_2.
+Proof.
+  pre_process.
+  rewrite H1.
+  unfold store_term at 2.
+  fold store_term.
+  Exists v_2 v.
+  entailer!.
+  sep_apply store_term_fold_out.
+  entailer!.
+
+  unfold store_imply_res.
+  unfold sep_impl.
+  destruct lt.
+
+  - entailer!.
+  - entailer!.
+  - contradiction.
+  - entailer!.
+  - lia.
+Qed.
+
+Lemma proof_of_separate_imply_return_wit_3 : separate_imply_return_wit_3.
+Proof.
+  pre_process.
+  rewrite H4.
+  unfold store_term at 3.
+  fold store_term.
+  rewrite H1.
+  unfold store_term at 3.
+  fold store_term.
+  Exists v_2 v v_4 v_3.
+
+  sep_apply ((store_term_fold_out v_4 ll) H0).
+  entailer!.
+
+  unfold store_imply_res.
+  unfold sep_impl.
+  destruct ll.
+  - entailer!.
+  - contradiction.
+  - entailer!.
+  - entailer!.
+Qed.
+
+Lemma proof_of_separate_imply_return_wit_4 : separate_imply_return_wit_4.
+Proof.
+  pre_process.
+  rewrite H6.
+  unfold store_term at 3.
+  fold store_term.
+  Exists v_2 v.
+  entailer!.
+
+  rewrite H3.
+  unfold store_term at 2.
+  fold store_term.
+  Exists v_4 v_3.
+  entailer!.
+
+  rewrite H0.
+  unfold store_term.
+  entailer!.
+
+  unfold store_imply_res.
+  unfold sep_impl.
+  destruct llctype.
+  - entailer!.
+  - entailer!.
+  - entailer!.
+  - entailer!.
+  - entailer!.
+  - entailer!.
+  - entailer!.
+  - contradiction.
+Qed. 
+
+Lemma proof_of_separate_imply_return_wit_5 : separate_imply_return_wit_5.
+Proof.
+  pre_process.
+  unfold store_imply_res.
+  unfold sep_impl.
+  rewrite H6.
+  rewrite H3.
+  rewrite H0.
+  unfold ctID in H.
+  destruct llctype; try lia.
+  Exists t1' t2'.
+  unfold store_term.
+  fold store_term.
+  Exists v_2 v.
+  Exists v_4 v_3.
+  entailer!.
+Qed.
+
+Lemma proof_of_separate_imply_which_implies_wit_1 : separate_imply_which_implies_wit_1.
+Proof.
+  pre_process.
+  sep_apply store_term_unfold.
+  unfold NULL.
+  entailer!.
+Qed.
+
+Lemma proof_of_separate_imply_which_implies_wit_2 : separate_imply_which_implies_wit_2.
+Proof.
+  pre_process.
+  sep_apply store_term'_Apply; unfold NULL in *.
+  Intros lt rt y z.
+  Exists z y lt rt.
+  rewrite H3.
+  entailer!.
+  lia.
+  lia.
+Qed.
+
+Lemma proof_of_separate_imply_which_implies_wit_3 : separate_imply_which_implies_wit_3.
+Proof.
+  pre_process.
+  sep_apply store_term_unfold.
+  unfold NULL.
+  entailer!.
+Qed.
+
+
+Lemma proof_of_separate_imply_which_implies_wit_4 : separate_imply_which_implies_wit_4.
+Proof.
+  pre_process.
+  sep_apply store_term'_Apply; unfold NULL in *.
+  Intros ll lr y z.
+  Exists z y ll lr.
+  entailer!.
+  lia.
+  lia.
+Qed. 
+
+Lemma proof_of_separate_imply_which_implies_wit_5 : separate_imply_which_implies_wit_5.
+Proof.
+  pre_process.
+  sep_apply store_term_unfold.
+  unfold NULL.
+  entailer!.
+Qed.
+
+Lemma proof_of_separate_imply_which_implies_wit_6 : separate_imply_which_implies_wit_6.
+Proof.
+  pre_process.
+  sep_apply store_term'_Const; unfold NULL in *.
+  Intros ty ct.
+  Exists ty ct.
+  rewrite <- H3.
+  entailer!.
+  lia.
+  lia.
+Qed. 
+
+Lemma proof_of_check_list_gen_entail_wit_1 : check_list_gen_entail_wit_1.
+Proof.
+  pre_process.
+  Exists theo nil.
+  entailer!.
+  unfold sllbseg_term_list, sllbseg.
+  entailer!.
+Qed.
+
+
+Lemma store_term_cell_fold: forall x y t,
+  x <> NULL ->
+  &(x # "term_list" ->ₛ "element") # Ptr |-> y **
+  store_term y t |--
+  store_term_cell x t.
+Proof.
+  intros.
+  unfold store_term_cell.
+  Exists y.
+  entailer!.
+Qed.
+
+Lemma sllbseg_one: forall a y retval,
+  retval <> NULL ->
+  y # Ptr |-> retval **
+  store_term_cell retval a |--
+  sllbseg_term_list y &(retval # "term_list" ->ₛ "next") (a::nil).
+Proof.
+  unfold sllbseg_term_list, sllbseg.
+  intros.
+  Exists retval.
+  entailer!.
+Qed.
+
+Lemma sllbseg_seg: forall x y z l1 l2,
+  sllbseg_term_list x y l1 **
+  sllbseg_term_list y z l2 |--
+  sllbseg_term_list x z (l1++l2).
+Proof.
+  intros.
+  revert x; induction l1; simpl; intros.
+  + entailer!.
+  subst x.
+  entailer!.
+  + Intros u.
+  Exists u.
+  entailer!.
+Qed.
+
+Lemma sllbseg_one_app: forall a l x y z retval,
+  retval <> NULL ->
+  sllbseg_term_list x y l **
+  y # Ptr |-> retval **
+  &(retval # "term_list" ->ₛ "element") # Ptr |-> z **
+  store_term z a |--
+  sllbseg_term_list x &(retval # "term_list" ->ₛ "next") (l++(a::nil)).
+Proof.
+  intros.
+  sep_apply (store_term_cell_fold retval z a); [ | auto].
+  sep_apply sllbseg_one; [ | auto].
+  sep_apply (sllbseg_seg x y &( retval # "term_list" ->ₛ "next") l (a :: nil)).
+  entailer!.
+Qed.
+
+Lemma proof_of_check_list_gen_entail_wit_2 : check_list_gen_entail_wit_2.
+Proof.
+  pre_process.
+  Exists tr (l_2 ++ (r::nil)).
+  entailer!.
+  + sep_apply sllbseg_one_app; [ entailer! | auto].
+  + subst.
+    clear - H4 H3.
+    unfold check_from_mid_rel in *.
+    rewrite (repeat_break_unfold _ _) in H4.
+    prove_by_one_abs_step (by_continue (tr, targ, l_2 ++ r :: nil)).
+    unfold check_list_gen_body.
+    unfold term_alpha_eqn in H3.
+    destruct term_alpha_eq; [ lia | ].
+    unfold sep_impl.
+    abs_ret_step.
+Qed.
+
+Lemma store_imply_res_zero: forall t,
+  store_imply_res 0 (sep_impl t) |-- [| sep_impl t = None |] && [|0 = NULL|] && emp.
+Proof.
+  intros.
+  remember (sep_impl t) as r.
+  unfold sep_impl in Heqr.
+  destruct t; try simpl.
+  + unfold store_imply_res; subst; entailer!.
+  + unfold store_imply_res; subst; entailer!.
+  + unfold store_imply_res.
+    destruct r; [ | entailer!].
+    destruct i; Intros x y.
+    destruct t1; try congruence.
+    destruct t1_1; try congruence.
+    destruct ctype; try congruence.
+    unfold store_ImplyProp.
+    entailer!.
+  + unfold store_imply_res; subst; entailer!.
+Qed.
+
+Lemma proof_of_check_list_gen_return_wit_1 : check_list_gen_return_wit_1.
+Proof.
+  pre_process.
+  subst.
+  sep_apply store_imply_res_zero.
+  Exists t_2 nil.
+  simpl; entailer!.
+  unfold check_from_mid_rel in *.
+  rewrite (repeat_break_unfold _ _) in H2.
+  prove_by_one_abs_step (by_break (makepair t_2 nil)).
+  unfold check_list_gen_body.
+  unfold term_alpha_eqn in H1.
+  destruct term_alpha_eq eqn:Heq; [ congruence | ].
+  rewrite H.
+  abs_ret_step.
+Qed.
+
+Lemma proof_of_check_list_gen_return_wit_2 : check_list_gen_return_wit_2.
+Proof.
+  pre_process.
+  Exists t_2 l_2.
+  entailer!.
+  unfold check_from_mid_rel in *.
+  rewrite (repeat_break_unfold _ _) in H1.
+  prove_by_one_abs_step (by_break (makepair t_2 l_2)).
+  unfold check_list_gen_body.
+  unfold term_alpha_eqn in H0.
+  destruct term_alpha_eq eqn:Heq; [ | congruence].
+  abs_ret_step.
+Qed.
+
+Lemma sllbseg_2_sllseg_term: forall x y l,
+  sllbseg_term_list x y l ** y # Ptr |-> 0 |--
+  EX h, x # Ptr |-> h ** sll_term_list h l.
+Proof.
+  intros.
+  unfold sllbseg_term_list, sll_term_list.
+  sep_apply (sllbseg_2_sllseg store_term_cell).
+  Intros h; Exists h.
+  sep_apply (sllseg_0_sll store_term_cell).
+  entailer!.
+Qed.
+
+Lemma proof_of_check_list_gen_which_implies_wit_1 : check_list_gen_which_implies_wit_1.
+Proof.
+  pre_process.
+  sep_apply sllbseg_2_sllseg_term.
+  Intros c; Exists c; entailer!.
+Qed.
+
+Lemma proof_of_check_list_gen_which_implies_wit_2 : check_list_gen_which_implies_wit_2.
+Proof.
+  pre_process.
+  unfold store_imply_res.
+  destruct (sep_impl ttm) eqn:Heq; [ | entailer!].
+  destruct i.
+  Intros y z.
+  unfold sep_impl in Heq.
+  destruct ttm eqn:Heq1; try congruence.
+  destruct t1 eqn:Heq11; try congruence.
+  destruct t3 eqn:Heq111; try congruence.
+  destruct ctype eqn:Hc; try congruence.
+  unfold store_ImplyProp.
+  Exists z y content t4 t2.
+  inversion Heq.
+  entailer!.
+Qed.
+
+Lemma proof_of_check_list_gen_which_implies_wit_3 : check_list_gen_which_implies_wit_3.
+Proof.
+  pre_process.
+  unfold store_ImplyProp.
+  entailer!.
+Qed.
+
+Lemma proof_of_check_list_gen_which_implies_wit_4 : check_list_gen_which_implies_wit_4.
+Proof.
+  pre_process.
+  sep_apply sllbseg_2_sllseg_term.
+  Intros c; Exists c; entailer!.
+Qed.
